@prefix rdf: <http://www.w3.org/1999/02/22-rdf-syntax-ns#> .
@prefix rdfs: <http://www.w3.org/2000/01/rdf-schema#> .
@prefix : <http://kloud.one/ud2rdf#>.

# super class
:Edge rdf:type rdfs:Class .
:Node rdf:type rdfs:Class .   

# 1.1 - Nsubj
:Nsubj rdfs:subClassOf :Edge ;
        rdfs:label "nsubj"@en ;
        rdfs:comment "Подлежащее"@ru ;
        rdfs:comment "A nominal subject (nsubj) is a nominal which is the syntactic subject and the proto-agent of a clause."@en .

# 1.2 - Nsubj:pass
:Nsubj_pass rdfs:subClassOf :Edge ;
        rdfs:label "nsubj:pass"@en ;
        rdfs:comment "Подлежащее"@ru ;
        rdfs:comment "A nominal subject (nsubj) is a nominal which is the syntactic subject and the proto-agent of a clause."@en .

# 2 - obj
:Obj rdfs:subClassOf :Edge ;
        rdfs:label "obj"@en ;
        rdfs:comment "Прямое дополнение"@ru ;
        rdfs:comment "The object of a verb is the second most core argument of a verb after the subject."@en .

# 3 - Iobj
:Iobj rdfs:subClassOf :Edge ;
        rdfs:label "iobj"@en ;
        rdfs:comment "Косвенное дополнение"@ru ;
        rdfs:comment "The indirect object of a verb is any nominal phrase that is a core argument of the verb but is not its subject or (direct) object."@en .

# 4 - Obl
:Obl rdfs:subClassOf :Edge ;
        rdfs:label "obl"@en ;
        rdfs:comment "Обстоятельство"@ru ;
        rdfs:comment "The obl relation is used for a nominal (noun, pronoun, noun phrase) functioning as a non-core (oblique) argument or adjunct."@en .

# 5 - Vocative
:Vocative rdfs:subClassOf :Edge ;
        rdfs:label "vocative"@en ;
        rdfs:comment "Обращение"@ru ;
        rdfs:comment "The vocative relation is used to mark a dialogue participant addressed in a text (common in conversations, dialogue, emails, newsgroup postings, etc.)."@en .

# 6 - Expl
:Expl rdfs:subClassOf :Edge ;
        rdfs:label "expl"@en ;
        rdfs:comment "Присловье"@ru ;
        rdfs:comment "This relation captures expletive or pleonastic nominals."@en .

# 7 - Dislocated ОТСУТСТВУЕТ
:Dislocated rdfs:subClassOf :Edge ;
        rdfs:label "dislocated"@en ;
        rdfs:comment ""@ru ;
        rdfs:comment ""@en .

# 8 - Nmod
:Nmod rdfs:subClassOf :Edge ;
        rdfs:label "nmod"@en ;
        rdfs:comment "Зависимость существительного от существительного (дополнение, определение, обстоятельство)"@ru ;
        rdfs:comment "The nmod relation is used for nominal dependents of another noun or noun phrase and functionally corresponds to an attribute, or genitive complement."@en .

# 9 - Appos
:Appos rdfs:subClassOf :Edge ;
        rdfs:label "appos"@en ;
        rdfs:comment "Приложение"@ru ;
        rdfs:comment "An appositional modifier of a noun is a nominal immediately following the first noun that serves to define, modify, name, or describe that noun."@en .

# 10.1 - Nummod
:Nummod rdfs:subClassOf :Edge ;
        rdfs:label "nummod"@en ;
        rdfs:comment "Числительное"@ru ;
        rdfs:comment "A numeric modifier of a noun is any number phrase that serves to modify the meaning of the noun with a quantity."@en .

# 10.2 - Nummod:gov
:Nummod_gov rdfs:subClassOf :Edge ;
        rdfs:label "nummod:gov"@en ;
        rdfs:comment "Числительное"@ru ;
        rdfs:comment "A numeric modifier of a noun is any number phrase that serves to modify the meaning of the noun with a quantity."@en .

# 10.2 - Nummod:entity
:Nummod_entity rdfs:subClassOf :Edge ;
        rdfs:label "nummod:entity"@en ;
        rdfs:comment "Числительное"@ru ;
        rdfs:comment "A numeric modifier of a noun is any number phrase that serves to modify the meaning of the noun with a quantity."@en .


# 11.1 - Csubj
:Csubj rdfs:subClassOf :Edge ;
        rdfs:label "csubj"@en ;
        rdfs:comment "Клаузальный субъект"@ru ;
        rdfs:comment "A clausal subject is a clausal syntactic subject of a clause, i.e., the subject is itself a clause."@en .

# 11.2 - Csubj:pass
:Csubj_pass rdfs:subClassOf :Edge ;
        rdfs:label "csubj:pass"@en ;
        rdfs:comment "Клаузальный субъект"@ru ;
        rdfs:comment "A clausal subject is a clausal syntactic subject of a clause, i.e., the subject is itself a clause."@en .

# 12 - Ccomp
:Ccomp rdfs:subClassOf :Edge ;
        rdfs:label "ccomp"@en ;
        rdfs:comment "Клаузальное дополнение"@ru ;
        rdfs:comment "A clausal complement of a verb or adjective is a dependent clause which is a core argument."@en .

# 13 - Xcomp
:Xcomp rdfs:subClassOf :Edge ;
        rdfs:label "xcomp"@en ;
        rdfs:comment "Инфинитив"@ru ;
        rdfs:comment "An open clausal complement (xcomp) of a verb or an adjective is a predicative or clausal complement without its own subject."@en .

# 14 - Advcl
:Advcl rdfs:subClassOf :Edge ;
        rdfs:label "advcl"@en ;
        rdfs:comment "Клаузальное обстоятельство"@ru ;
        rdfs:comment "An adverbial clause modifier is a clause which modifies a verb or other predicate (adjective, etc.), as a modifier not as a core complement."@en .

# 15.1 - Acl
:Acl rdfs:subClassOf :Edge ;
        rdfs:label "acl"@en ;
        rdfs:comment "Клаузальное определение"@ru ;
        rdfs:comment "Acl stands for finite and non-finite clauses that modify a nominal."@en .

# 15.2 - Acl:relcl
:Acl_relcl rdfs:subClassOf :Edge ;
        rdfs:label "acl:relcl"@en ;
        rdfs:comment "Клаузальное определение со словом 'который'"@ru ;
        rdfs:comment "Acl stands for finite and non-finite clauses that modify a nominal."@en .

# 16 - Advmod
:Advmod rdfs:subClassOf :Edge ;
        rdfs:label "advmod"@en ;
        rdfs:comment "Обстоятельственный модификатор"@ru ;
        rdfs:comment "An adverbial modifier of a word is a (non-clausal) adverb or adverbial phrase that serves to modify a predicate or a modifier word."@en .

# 17 - Discourse
:Discourse rdfs:subClassOf :Edge ;
        rdfs:label "discourse"@en ;
        rdfs:comment "Частицы и междометия"@ru ;
        rdfs:comment "This is used for interjections and other discourse particles and elements (which are not clearly linked to the structure of the sentence, except in an expressive way)."@en .

# 18 - Amod
:Amod rdfs:subClassOf :Edge ;
        rdfs:label "amod"@en ;
        rdfs:comment "Определение, выраженное прилагательным"@ru ;
        rdfs:comment "An adjectival modifier of a noun is any adjectival phrase that serves to modify the meaning of the noun."@en .

# 19.1 - Aux
:Aux rdfs:subClassOf :Edge ;
        rdfs:label "aux"@en ;
        rdfs:comment "Глагол-связка в составе сложного сказуемого"@ru ;
        rdfs:comment "n aux (auxiliary) of a clause is a function word associated with a verbal predicate that expresses categories such as tense, mood, aspect, voice or evidentiality."@en .

# 19.2 - Aux:pass
:Aux_pass rdfs:subClassOf :Edge ;
        rdfs:label "aux:pass"@en ;
        rdfs:comment "Глагол-связка в составе сложного сказуемого"@ru ;
        rdfs:comment "n aux (auxiliary) of a clause is a function word associated with a verbal predicate that expresses categories such as tense, mood, aspect, voice or evidentiality."@en .

# 20 - Cop
:Cop rdfs:subClassOf :Edge ;
        rdfs:label "cop"@en ;
        rdfs:comment "Глагол-связка в составе сложного сказуемого"@ru ;
        rdfs:comment "A cop (copula) is the relation of a function word used to link a subject to a nonverbal predicate."@en .

# 21 - Mark
:Mark rdfs:subClassOf :Edge ;
        rdfs:label "mark"@en ;
        rdfs:comment "Подчинительная клауза"@ru ;
        rdfs:comment "A marker is the word introducing a finite clause subordinate to another clause."@en .

# 21 - Det
:Det rdfs:subClassOf :Edge ;
        rdfs:label "det"@en ;
        rdfs:comment "Артикль"@ru ;
        rdfs:comment "The relation determiner (det) holds between a nominal head and its determiner."@en .

# 22 - Clf ОТСУТСТВУЕТ
:Clf rdfs:subClassOf :Edge ;
        rdfs:label "clf"@en ;
        rdfs:comment ""@ru ;
        rdfs:comment ""@en .

# 23 - Case
:Case rdfs:subClassOf :Edge ;
        rdfs:label "case"@en ;
        rdfs:comment "Падеж"@ru ;
        rdfs:comment "The case relation is used for any case-marking element which is treated as a separate syntactic word (including prepositions, postpositions, and clitic case markers)."@en .

# 24 - Conj
:Conj rdfs:subClassOf :Edge ;
        rdfs:label "conj"@en ;
        rdfs:comment "Союз (токены, соединённые им)"@ru ;
        rdfs:comment "A conjunct is the relation between two elements connected by a coordinating conjunction, such as and, or, etc."@en .

# 25 - Cc
:Cc rdfs:subClassOf :Edge ;
        rdfs:label "cc"@en ;
        rdfs:comment "Сочинительный союз"@ru ;
        rdfs:comment "A cc is the relation between a conjunct and a preceding coordinating conjunction."@en .

# 26 - Fixed
:Fixed rdfs:subClassOf :Edge ;
        rdfs:label "fixed"@en ;
        rdfs:comment "Устоявшееся сочетание слов"@ru ;
        rdfs:comment "The fixed relation is one of the three relations for multiword expressions (MWEs) (the other two being flat and compound)."@en .

# 27.1 - Flat
:Flat rdfs:subClassOf :Edge ;
        rdfs:label "flat"@en ;
        rdfs:comment "Связь именованных сущностей"@ru ;
        rdfs:comment "TThe flat relation is one of three relations for multiword expressions multiword expressions (MWEs) in UD (the other two being fixed and compound). It is used for exocentric (headless) semi-fixed MWEs like names (Hillary Rodham Clinton) and dates (24 December)."@en .

# 27.2 - Flat:name
:Flat_name rdfs:subClassOf :Edge ;
        rdfs:label "flat:name"@en ;
        rdfs:comment "Связь именованных сущностей"@ru ;
        rdfs:comment "TThe flat relation is one of three relations for multiword expressions multiword expressions (MWEs) in UD (the other two being fixed and compound). It is used for exocentric (headless) semi-fixed MWEs like names (Hillary Rodham Clinton) and dates (24 December)."@en .

# 27.3 - Flat:foreign
:Flat_foreign rdfs:subClassOf :Edge ;
        rdfs:label "flat:foreign"@en ;
        rdfs:comment "Связь именованных сущностей"@ru ;
        rdfs:comment "TThe flat relation is one of three relations for multiword expressions multiword expressions (MWEs) in UD (the other two being fixed and compound). It is used for exocentric (headless) semi-fixed MWEs like names (Hillary Rodham Clinton) and dates (24 December)."@en .

# 28 - Compound
:Compound rdfs:subClassOf :Edge ;
        rdfs:label "compound"@en ;
        rdfs:comment "Сложные слова"@ru ;
        rdfs:comment "It is used for any kind of such compounding: noun compounds (e.g., phone book), but also verb and adjective compounds that are more common in other languages (such as Persian or Japanese light verb constructions)."@en .

# 29 - List
:List rdfs:subClassOf :Edge ;
        rdfs:label "list"@en ;
        rdfs:comment ""@ru ;
        rdfs:comment ""@en .

# 30 - Parataxis
:Parataxis rdfs:subClassOf :Edge ;
        rdfs:label "parataxis"@en ;
        rdfs:comment "Паратаксис"@ru ;
        rdfs:comment "The parataxis relation (from Greek for “place side by side”) is a relation between a word (often the main predicate of a sentence) and other elements, such as a sentential parenthetical or a clause after a “:” or a “;”, placed side by side without any explicit coordination, subordination, or argument relation with the head word. Parataxis is a discourse-like equivalent of coordination, and so usually obeys an iconic ordering."@en .

# 31 - Orphan
:Orphan rdfs:subClassOf :Edge ;
        rdfs:label "orphan"@en ;
        rdfs:comment "Эллипсис"@ru ;
        rdfs:comment "The ‘orphan’ relation is used in cases of head ellipsis where simple promotion would result in unnatural and misleading dependency relation."@en .

# 32 - Goeswith
:Goeswith rdfs:subClassOf :Edge ;
        rdfs:label "goeswith"@en ;
        rdfs:comment ""@ru ;
        rdfs:comment ""@en .

# 33 - Reparandum
:Reparandum rdfs:subClassOf :Edge ;
        rdfs:label "reparandum"@en ;
        rdfs:comment ""@ru ;
        rdfs:comment ""@en .

# 34 - Punct
:Punct rdfs:subClassOf :Edge ;
        rdfs:label "punct"@en ;
        rdfs:comment "Пунктуационный знак"@ru ;
        rdfs:comment "This is used for any piece of punctuation in a clause, if punctuation is being retained in the typed dependencies."@en .

# 35 - Root
:Root rdfs:subClassOf :Edge ;
        rdfs:label "root"@en ;
        rdfs:comment "Корень"@ru ;
        rdfs:comment "The root grammatical relation points to the root of the sentence. A fake node ROOT is used as the governor."@en .

# 36 - Dep
:Dep rdfs:subClassOf :Edge ;
        rdfs:label "dep"@en ;
        rdfs:comment "Неопределённая связь"@ru ;
        rdfs:comment ""@en .

# root node
:root_node rdf:type :Node ;
        rdfs:label "root node"@en ;
        rdfs:comment "фиктивная вершина - начало графа предложения"@ru .

# blank node
:blank_node rdf:type :Node ;
        rdfs:label "blank node"@en ;
        rdfs:comment "фиктивная вершина графа предложения, blank node"@ru .